src/Examples/AtomicPair/RefinementShadow.v
@@ -3,8 +3,6 @@ Require Export CSL.Refinement.
 Require Import AtomicPairAPI AtomicPair.ImplShadow ExMach.WeakestPre ExMach.RefinementAdequacy.
 Unset Implicit Arguments.
 
-Definition recv : proc ExMach.Op _ := Ret tt.
-
 (* TODO: move *)
 Section ghost_var_helpers.
 Context {A: ofeT} `{@LeibnizEquiv _ A.(ofe_equiv)} `{OfeDiscrete A}.
@@ -30,6 +28,19 @@ Proof.
 Qed.
 End ghost_var_helpers.
 
+  (* Extends the iExist tactic to make it easier to re-prove invariants after steps *)
+Instance from_exist_left_sep {Σ} {A} (Φ : A → iProp Σ) Q :
+  FromExist (▷ (∃ a, Φ a) ∗ Q) (λ a, ▷ Φ a ∗ Q)%I .
+Proof. rewrite /FromExist. iIntros "H". iDestruct "H" as (?) "(?&$)". iExists _; eauto. Qed.
+
+
+Local Ltac destruct_einner H :=
+  iDestruct H as (? (?&?) (?&?)) ">(Hown1&Hown2&Hown3&Hsource&Hmap)";
+  iDestruct "Hmap" as "(Hptr&Hcase)";
+  try (iDestruct (ghost_var_agree with "Hown1 [$]") as %?; subst; []);
+  try (iDestruct (ghost_var_agree with "Hown2 [$]") as %Hp; inversion_clear Hp; subst; []);
+  try (iDestruct (ghost_var_agree with "Hown3 [$]") as %Hp; inversion_clear Hp; subst; []).
+
 Set Default Proof Using "Type".
 Section refinement_triples.
   Context `{!exmachG Σ, lockG Σ, !@cfgG (AtomicPair.Op) (AtomicPair.l) Σ,
@@ -39,7 +50,7 @@ Section refinement_triples.
 
   Import ExMach.
 
-  (* TODO: this should work, but the invariant is too global: ideally, 
+  (* TODO: this should work, but the invariant is too global: ideally,
      most threads should not care about the value in the non-pointed to
      copy, and a writer who holds the lock should be able to modify it freely
      without opening this invariant up prior to updating the pointer *)
@@ -57,7 +68,7 @@ Section refinement_triples.
             ∗ own γ3 (● (Excl' pother))
             ∗ source_state pcurr ∗
             ptr_map ptr_val pcurr pother)%I.
-            
+
 
   (* Holding the lock guarantees the value of the atomic pair/pointer will not
      change out from underneath you -- this is enforced by granting ownership of
@@ -76,31 +87,19 @@ Section refinement_triples.
     (∃ (ptr_val : nat) (pcurr: nat * nat) pother,
         source_state pcurr ∗ ptr_map ptr_val pcurr pother ∗ lock_addr m↦ 0)%I.
 
-
   Definition lN : namespace := (nroot.@"lock").
   Definition iN : namespace := (nroot.@"inner").
 
   Definition ExecInv :=
     (source_ctx ρ ∗ ∃ γlock γ1 γ2 γ3, is_lock lN γlock lock_addr (ExecLockInv γ1 γ2 γ3)
                                            ∗ inv iN (ExecInner γ1 γ2 γ3))%I.
+  Definition CrashInv := (source_ctx ρ ∗ inv iN CrashInner)%I.
 
-
-  (* Extends the iExist tactic to make it easier to re-prove invariants after steps *)
-  Instance from_exist_left_sep {A} (Φ : A → iProp Σ) Q :
-    FromExist (▷ (∃ a, Φ a) ∗ Q) (λ a, ▷ Φ a ∗ Q)%I .
-  Proof. rewrite /FromExist. iIntros "H". iDestruct "H" as (?) "(?&$)". iExists _; eauto. Qed.
-
-  Ltac destruct_einner H :=
-    iDestruct "H" as (? (?&?) (?&?)) ">(Hown1&Hown2&Hown3&Hsource&Hmap)";
-    iDestruct "Hmap" as "(Hptr&Hcase)";
-    try (iDestruct (ghost_var_agree with "Hown1 [$]") as %?; subst; []);
-    try (iDestruct (ghost_var_agree with "Hown2 [$]") as %Hp; inversion_clear Hp; subst; []);
-    try (iDestruct (ghost_var_agree with "Hown3 [$]") as %Hp; inversion_clear Hp; subst; []).
 
   Lemma read_of_swap ptr_val :
     (read_addrs (swap_ptr ptr_val)) = write_addrs ptr_val.
   Proof. destruct ptr_val => //=. Qed.
-  
+
   Lemma write_of_swap ptr_val :
     (write_addrs (swap_ptr ptr_val)) = read_addrs ptr_val.
   Proof. destruct ptr_val => //=. Qed.
@@ -142,7 +141,7 @@ Section refinement_triples.
     iMod (ghost_var_update γ3 (new_fst, new_snd) with "Hown3 [$]") as "(Hown3&Hother_ghost)".
     iModIntro; iExists _, _; iFrame.
     simpl.
-    iExists (_, _). iFrame. 
+    iExists (_, _). iFrame.
 
     (* iInv fails for mysterious type class reasons that I cannot debug *)
     wp_bind.
@@ -166,7 +165,235 @@ Section refinement_triples.
 
     iModIntro.
     iApply (wp_unlock with "[-HΦ Hj]"); iFrame.
-    { iFrame "Hlockinv". iExists _, _, _. iFrame. } 
+    { iFrame "Hlockinv". iExists _, _, _. iFrame. }
     iIntros "!> _". by iApply "HΦ".
   Qed.
+
+  Lemma read_refinement {T} j K `{LanguageCtx AtomicPair.Op (nat*nat) T AtomicPair.l K}:
+    {{{ j ⤇ K (Call (AtomicPair.Read)) ∗ ExecInv }}} read {{{ v, RET v; j ⤇ K (Ret v) }}}.
+  Proof.
+    iIntros (Φ) "(Hj&#Hsource_inv&Hinv) HΦ".
+    iDestruct "Hinv" as (γlock γ1 γ2 γ3) "(#Hlockinv&#Hinv)".
+    wp_bind. iApply (wp_lock with "[$]").
+    iIntros "!> (Hlocked&HEL)".
+    iDestruct "HEL" as (ptr_val pcurr pother) "(Hptr_ghost&Hpair_ghost&Hother_ghost)".
+    wp_bind.
+    iInv "Hinv" as "H".
+    destruct_einner "H".
+    iApply (wp_read_disk with "[$]"). iIntros "!> Haddr".
+    iModIntro; iExists _, _, _; iFrame.
+    wp_bind.
+    iInv "Hinv" as "H".
+    destruct_einner "H".
+    iDestruct "Hcase" as "(Hfst&Hsnd&?&?)".
+    iApply (wp_read_disk with "Hfst"). iIntros "!> Hfst".
+    iModIntro; iExists _, _, _; iFrame.
+    wp_bind.
+    iInv "Hinv" as "H".
+    destruct_einner "H".
+    iDestruct "Hcase" as "(Hfst&Hsnd&?&?)".
+    iApply (wp_read_disk with "Hsnd"). iIntros "!> Hsnd".
+    iMod (ghost_step_lifting with "Hj Hsource_inv Hsource") as "(Hj&Hsource&_)".
+    { do 2 eexists; split; last by eauto. econstructor. }
+    { solve_ndisj. }
+
+    iModIntro; iExists _, _, _; iFrame.
+    wp_bind.
+    iApply (wp_unlock with "[-HΦ Hj]"); iFrame.
+    { iFrame "Hlockinv". iExists _, _, _. iFrame. }
+    iIntros "!> _". simpl.
+    wp_ret. by iApply "HΦ".
+  Qed.
+
+  Lemma init_mem_split:
+    (([∗ map] i↦v ∈ init_zero, i m↦ v) -∗ lock_addr m↦ 0)%I.
+  Proof.
+    iIntros "Hmem".
+    rewrite (big_opM_delete _ _ 0 0); last first.
+    { rewrite /ExMach.mem_state. apply init_zero_lookup_lt_zero. rewrite /size. lia. }
+    iDestruct "Hmem" as "(?&_)".
+    iFrame.
+  Qed.
+
+  Lemma init_disk_split:
+    (([∗ map] i↦v ∈ init_zero, i d↦ v)
+       -∗ ptr_addr d↦ 0 ∗ copy0_fst d↦ 0 ∗ copy0_snd d↦ 0
+          ∗ copy1_fst d↦ 0 ∗ copy1_snd d↦ 0)%I.
+  Proof.
+    iIntros "Hdisk".
+    rewrite (big_opM_delete _ _ 0 0); last first.
+    { rewrite /ExMach.disk_state. apply init_zero_lookup_lt_zero. rewrite /size. lia. }
+    rewrite (big_opM_delete _ _ 1 0); last first.
+    { rewrite /ExMach.disk_state.
+      rewrite lookup_delete_ne; last auto.
+      apply init_zero_lookup_lt_zero. rewrite /size. lia. }
+    rewrite (big_opM_delete _ _ 2 0); last first.
+    { rewrite /ExMach.disk_state.
+      rewrite lookup_delete_ne; last auto.
+      rewrite lookup_delete_ne; last auto.
+      apply init_zero_lookup_lt_zero. rewrite /size. lia. }
+    rewrite (big_opM_delete _ _ 3 0); last first.
+    { rewrite /ExMach.disk_state.
+      rewrite lookup_delete_ne; last auto.
+      rewrite lookup_delete_ne; last auto.
+      rewrite lookup_delete_ne; last auto.
+      apply init_zero_lookup_lt_zero. rewrite /size. lia. }
+    rewrite (big_opM_delete _ _ 4 0); last first.
+    { rewrite /ExMach.disk_state.
+      rewrite lookup_delete_ne; last auto.
+      rewrite lookup_delete_ne; last auto.
+      rewrite lookup_delete_ne; last auto.
+      rewrite lookup_delete_ne; last auto.
+      apply init_zero_lookup_lt_zero. rewrite /size. lia. }
+    rewrite (big_opM_delete _ _ 5 0); last first.
+    { rewrite /ExMach.disk_state.
+      rewrite lookup_delete_ne; last auto.
+      rewrite lookup_delete_ne; last auto.
+      rewrite lookup_delete_ne; last auto.
+      rewrite lookup_delete_ne; last auto.
+      rewrite lookup_delete_ne; last auto.
+      apply init_zero_lookup_lt_zero. rewrite /size. lia. }
+    iDestruct "Hdisk" as "(?&?&?&?&?&_)".
+    iFrame.
+  Qed.
+
+
 End refinement_triples.
+
+Section refinement.
+
+  Definition helperΣ : gFunctors := #[GFunctor (authR (optionUR (exclR (natC))));
+                                       GFunctor (authR (optionUR (exclR (prodC natC natC))))].
+  Instance subG_helperΣ : subG helperΣ Σ → inG Σ (authR (optionUR (exclR (natC)))).
+  Proof. solve_inG. Qed.
+  Instance subG_helperΣ' : subG helperΣ Σ → inG Σ (authR (optionUR (exclR (prodC natC natC)))).
+  Proof. solve_inG. Qed.
+
+  Definition myΣ : gFunctors := #[Adequacy.exmachΣ; @cfgΣ AtomicPair.Op AtomicPair.l; lockΣ; helperΣ].
+  Existing Instance subG_cfgPreG.
+
+  Definition init_absr σ1a σ1c :=
+    ExMach.l.(initP) σ1c ∧ AtomicPair.l.(initP) σ1a.
+
+
+  Import ExMach.
+  Lemma exmach_crash_refinement_seq {T} σ1c σ1a (es: proc_seq AtomicPair.Op T) :
+    init_absr σ1a σ1c →
+    ¬ proc_exec_seq AtomicPair.l es (rec_singleton (Ret ())) σ1a Err →
+    ∀ σ2c res, ExMach.l.(proc_exec_seq) (compile_proc_seq ImplShadow.impl es)
+                                        (rec_singleton recv) σ1c (Val σ2c res) →
+    ∃ σ2a, AtomicPair.l.(proc_exec_seq) es (rec_singleton (Ret tt)) σ1a (Val σ2a res).
+  Proof.
+    eapply (exmach_crash_refinement_seq) with
+        (Σ := myΣ)
+        (exec_inv := fun H1 H2 => (∃ ρ, @ExecInv myΣ H2 _ H1 _ _ ρ)%I)
+        (crash_inv := fun H1 H2 =>(∃ ρ, @CrashInv myΣ H2 H1 ρ)%I)
+        (exec_inner := fun H1 H2 => (∃ v, lock_addr m↦ v ∗
+            (∃ γ1 γ2 γ3, (⌜ v = 0  ⌝ -∗ @ExecLockInv myΣ _ _ γ1 γ2 γ3) ∗ @ExecInner myΣ H2 H1 _ _ γ1 γ2 γ3))%I)
+        (crash_inner := fun H1 H2 => (@CrashInner myΣ H2 H1)%I)
+        (E := nclose sourceN).
+    { apply _. }
+    { apply _. }
+    { intros. apply _. }
+    { intros. apply _. }
+    { set_solver+. }
+    { intros. iIntros "(?&H)". iDestruct "H" as (ρ) "H". destruct op.
+      - iApply (write_refinement with "[$]"). eauto.
+      - iApply (read_refinement with "[$]"). eauto.
+    }
+    { intros. iIntros "H". iDestruct "H" as (ρ) "(?&?)". eauto. }
+    { intros. iIntros "H". iDestruct "H" as (ρ) "(#Hctx&#Hinv)".
+      wp_ret. iInv "Hinv" as (ptr_val pcurr pother) ">(?&Hcase&?)" "_".
+      iMod (own_alloc (● (Excl' ptr_val) ⋅ ◯ (Excl' ptr_val))) as (γ1) "[Hauth_ptr Hfrag_ptr]".
+      { apply auth_valid_discrete_2; split; eauto. econstructor. }
+      iMod (own_alloc (● (Excl' pcurr) ⋅ ◯ (Excl' pcurr))) as (γ2) "[Hauth_curr Hfrag_curr]".
+      { by eauto. }
+      iMod (own_alloc (● (Excl' pother) ⋅ ◯ (Excl' pother))) as (γ3) "[Hauth_other Hfrag_other]".
+      { by eauto. }
+      iApply (fupd_mask_weaken _ _).
+      { solve_ndisj. }
+      iExists pcurr, pcurr. iFrame.
+      iSplitL "".
+      { iPureIntro; econstructor. }
+      iClear "Hctx Hinv".
+      iIntros (???) "(#Hctx&Hstate)".
+      iModIntro. iExists _. iFrame. iExists γ1, γ2, γ3.
+      iSplitL "Hfrag_ptr Hfrag_curr Hfrag_other"; iIntros; iExists _, _, _; iFrame.
+    }
+    { intros ?? (H&?). inversion H. subst. eapply ExMach.init_state_wf. }
+    { intros ??? (H&Hinit) ??. inversion H. inversion Hinit. subst.
+      iIntros "(Hmem&Hdisk&#?&Hstate)".
+      iMod (own_alloc (● (Excl' 0) ⋅ ◯ (Excl' 0))) as (γ1) "[Hauth_ptr Hfrag_ptr]".
+      { apply auth_valid_discrete_2; split; eauto. econstructor. }
+      iMod (own_alloc (● (Excl' (0, 0)) ⋅ ◯ (Excl' (0, 0)))) as (γ2) "[Hauth_curr Hfrag_curr]".
+      { apply auth_valid_discrete_2; split; eauto. econstructor. }
+      iMod (own_alloc (● (Excl' (0, 0)) ⋅ ◯ (Excl' (0, 0)))) as (γ3) "[Hauth_other Hfrag_other]".
+      { apply auth_valid_discrete_2; split; eauto. econstructor. }
+      iPoseProof (init_mem_split with "Hmem") as "?".
+      iPoseProof (init_disk_split with "Hdisk") as "(?&?&?&?&?)".
+      iModIntro. iExists _. iFrame. iExists γ1, γ2, γ3.
+      iSplitL "Hfrag_ptr Hfrag_curr Hfrag_other"; iIntros; iExists _, _, _; iFrame.
+      simpl. iFrame.
+    }
+    { intros. iIntros "H". iDestruct "H" as (ρ) "(#Hctx&#Hinv)".
+      iDestruct "Hinv" as (γlock γ1 γ2 γ3) "(#Hlock&#Hinv)".
+      iInv "Hinv" as "Hopen" "_".
+      destruct_einner "Hopen".
+      iApply fupd_mask_weaken; first by solve_ndisj.
+      iIntros (?) "Hmem".
+      iModIntro. iExists _, _, _. iFrame.
+      iPoseProof (@init_mem_split with "Hmem") as "?".
+      iFrame.
+    }
+    { intros. iIntros "H". iDestruct "H" as (ρ) "(#Hctx&#Hinv)".
+      iInv "Hinv" as ">Hopen" "_".
+      iDestruct "Hopen" as (???) "(?&?&_)".
+      iApply fupd_mask_weaken; first by solve_ndisj.
+      iIntros (?) "Hmem".
+      iModIntro. iExists _, _, _. iFrame.
+      iPoseProof (@init_mem_split with "Hmem") as "?".
+      iFrame.
+    }
+    { intros. iIntros "H". iDestruct "H" as "(Hinv&#Hsrc)".
+      iDestruct "Hinv" as (invG) "Hinv".
+      iDestruct "Hinv" as (???) "(?&?&?)".
+      iMod (@inv_alloc myΣ (exm_invG) iN _ CrashInner with "[-]").
+      { iNext. iExists _, _, _; iFrame. }
+      iModIntro. iExists _. iFrame "Hsrc". auto.
+    }
+    { intros. iIntros "H". iDestruct "H" as "(Hinv&#Hsrc)".
+      iDestruct "Hinv" as (invG v) "Hinv".
+      iDestruct "Hinv" as "(?&Hinv)".
+      iDestruct "Hinv" as (γ1 γ2 γ3) "(Hlock&Hinner)".
+      iMod (@lock_init myΣ (ExMachG _ (exm_invG) (exm_mem_inG) (exm_disk_inG)) _ lN
+                       lock_addr _ (ExecLockInv γ1 γ2 γ3) with "[$] [-Hinner]") as (γlock) "H".
+      { iFrame. }
+      iMod (@inv_alloc myΣ (exm_invG) iN _ (ExecInner γ1 γ2 γ3) with "[Hinner]").
+      { iFrame. }
+      iModIntro. iExists cfg. iFrame "Hsrc". iExists _, _, _, _. iFrame.
+    }
+    { iIntros (??) "H".
+      iDestruct "H" as (?) "(?&H)".
+      iDestruct "H" as (????) "(?&Hinv)".
+      iInv "Hinv" as "H" "_".
+      destruct_einner "H".
+      iApply fupd_mask_weaken; first by solve_ndisj.
+      iExists _; iFrame.
+    }
+    { iIntros (??) "H".
+      iDestruct "H" as (?) "(?&H)".
+      iDestruct "H" as (????) "(Hlock&Hinv)".
+      iInv "Hinv" as "H" "_".
+      destruct_einner "H".
+      iMod (lock_crack with "Hlock") as ">H"; first by solve_ndisj.
+      iDestruct "H" as (v) "(?&?)".
+      iApply fupd_mask_weaken; first by solve_ndisj.
+      iExists _; iFrame.
+      iFrame. iIntros (???) "(?&?)".
+      iModIntro.
+      iExists _. iFrame. iExists _, _, _. iFrame.
+      iExists _, _, _. iFrame.
+    }
+  Qed.
+
+End refinement.
